Apply the framework to the StatDB example to show that the impl gives refinements.
The notion of refinement here is only about final observable behavior (so far),
not trace outputs.

It is very verbose for such a trivial example, but there are some re-usable
patterns that could be extracted out, and part of this is some 'standard
boilerplate' -- the relative costs of which will not seem so bad for more
serious examples (hopefully).

This result still depends on one admit in the generic CSL adequcy theorem.
Namely, one that shows the compiled program has no errors -- but I know how to
prove that.

src/Examples/StatDb/Refinement.v
@@ -1,44 +1,69 @@
-From iris.algebra Require Import auth gmap.
+From iris.algebra Require Import auth gmap list.
 Require Export CSL.Refinement.
-Require Import StatDb.Impl ExMach.WeakestPre.
+Require Import StatDb.Impl ExMach.WeakestPre ExMach.RefinementAdequacy.
 Set Default Proof Using "Type".
 Unset Implicit Arguments.
 
+Definition recv : proc ExMach.Op _ := Ret tt.
 
 
 Section refinement_triples.
-  Context `{!exmachG Σ, !lockG Σ, !@cfgG (DB.Op) (DB.l) Σ}.
+  Context `{!exmachG Σ, lockG Σ, !@cfgG (DB.Op) (DB.l) Σ, !inG Σ (authR (optionUR (exclR (listC natC))))}.
   Context (ρ : thread_pool DB.Op * DB.l.(State)).
 
   Import ExMach.
 
-  Definition DBLockInv :=
-    (∃ l, source_state l
+  Definition DBInnerInv γ :=
+    (∃ (l: list nat), own γ (● (Excl' l)) ∗ source_state l)%I.
+  Definition DBLockInv γ :=
+    (∃ (l: list nat), own γ (◯ (Excl' l))
           ∗ sum_addr m↦ (fold_right plus O l)
           ∗ count_addr m↦ (length l))%I.
+  Definition DBCrashInner :=
+    (∃ l, source_state l
+          ∗ lock_addr m↦ O
+          ∗ sum_addr m↦ O
+          ∗ count_addr m↦ O)%I.
 
-  Definition DBInv := (source_ctx ρ ∗ ∃ N γ, is_lock N γ lock_addr DBLockInv)%I.
+  Definition lN : namespace := (nroot.@"lock").
+  Definition iN : namespace := (nroot.@"inner").
+
+  Definition DBInv := (source_ctx ρ ∗
+                                  ∃ γ1 γ2, is_lock lN γ1 lock_addr (DBLockInv γ2)
+                                                   ∗ inv iN (DBInnerInv γ2))%I.
+  Definition CrashInv := (source_ctx ρ ∗ inv iN DBCrashInner)%I.
 
   (* TODO: write smart tactics for applying the wp_primitives *)
   Lemma add_refinement {T} j K `{LanguageCtx DB.Op unit T DB.l K} n:
     {{{ j ⤇ K (Call (DB.Add n)) ∗ DBInv }}} add n {{{ v, RET v; j ⤇ K (Ret v) }}}.
   Proof.
     iIntros (Φ) "(Hj&#Hsource_inv&Hinv) HΦ".
-    iDestruct "Hinv" as (N γ) "#Hinv".
+    iDestruct "Hinv" as (γ1 γ2) "(#Hlockinv&#Hinv)".
     wp_bind. iApply (wp_lock with "[$]").
     iIntros "!> (Hlocked&HDB)".
-    iDestruct "HDB" as (l) "(Hsource&Hsum&Hcount)".
+    iDestruct "HDB" as (l) "(Hsource_tok&Hsum&Hcount)".
     wp_bind. iApply (wp_read_mem with "Hsum"). iIntros "!> Hsum".
     wp_bind. iApply (wp_write_mem with "[$]"). iIntros "!> Hsum".
     wp_bind. iApply (wp_read_mem with "Hcount"). iIntros "!> Hcount".
-    wp_bind. iApply (wp_write_mem with "[$]"). iIntros "!> Hcount".
+    wp_bind.
+    iInv "Hinv" as (l') ">(Htok&Hsource)".
+    iDestruct (own_valid_2 with "Htok Hsource_tok")
+      as %[<-%Excl_included%leibniz_equiv _]%auth_valid_discrete_2.
     iMod (ghost_step_lifting with "Hj Hsource_inv Hsource") as "(Hj&Hsource&_)".
     { do 2 eexists; split; last by eauto. econstructor. }
-    { set_solver+. }
-    iAssert DBLockInv with "[-HΦ Hlocked Hj]" as "HDB".
-    { iExists _; iFrame. }
+    { solve_ndisj. }
+    iMod (own_update_2 _ _ _ (● Excl' (n :: l) ⋅ ◯ Excl' (n :: l)) with "Htok Hsource_tok")
+      as "[Hfull ?]".
+    { by apply auth_update, option_local_update, exclusive_local_update. }
+
+    iApply (wp_write_mem with "[$]"). iIntros "!> Hcount".
+    iModIntro.
+    iSplitL "Hfull Hsource".
+    { iNext. iExists _. iFrame. }
+    iAssert (DBLockInv γ2) with "[-HΦ Hlocked Hj]" as "HDB".
+    { iExists _; simpl. do 2 iFrame. }
     iApply (wp_unlock with "[-HΦ Hj]"); iFrame.
-    { iFrame "Hinv"; eauto. }
+    { iFrame "Hlockinv". eauto. }
     iIntros "!> _". by iApply "HΦ".
   Qed.
 
@@ -46,83 +71,175 @@ Section refinement_triples.
     {{{ j ⤇ K (Call (DB.Avg)) ∗ DBInv }}} avg {{{ n, RET n; j ⤇ K (Ret n) }}}.
   Proof.
     iIntros (Φ) "(Hj&#Hsource_inv&Hinv) HΦ".
-    iDestruct "Hinv" as (N γ) "#Hinv".
+    iDestruct "Hinv" as (γ1 γ2) "(#Hlockinv&#Hinv)".
     wp_bind. iApply (wp_lock with "[$]").
     iIntros "!> (Hlocked&HDB)".
-    iDestruct "HDB" as (l) "(Hsource&Hsum&Hcount)".
+    iDestruct "HDB" as (l) "(Hsource_tok&Hsum&Hcount)".
     wp_bind. iApply (wp_read_mem with "Hsum"). iIntros "!> Hsum".
-    wp_bind. iApply (wp_read_mem with "Hcount"). iIntros "!> Hcount".
+    wp_bind.
+    iInv "Hinv" as (l') ">(Htok&Hsource)".
+    iDestruct (own_valid_2 with "Htok Hsource_tok")
+      as %[<-%Excl_included%leibniz_equiv _]%auth_valid_discrete_2.
     iMod (ghost_step_lifting with "Hj Hsource_inv Hsource") as "(Hj&Hsource&_)".
     { do 2 eexists; split; last by eauto. econstructor. }
-    { set_solver+. }
-    iAssert DBLockInv with "[-HΦ Hlocked Hj]" as "HDB".
+    { solve_ndisj. }
+
+    iApply (wp_read_mem with "Hcount"). iIntros "!> Hcount".
+    iModIntro.
+    iSplitL "Htok Hsource".
+    { iNext. iExists _. iFrame. }
+    iAssert (DBLockInv γ2) with "[-HΦ Hlocked Hj]" as "HDB".
     { iExists _; iFrame. }
     wp_bind. iApply (wp_unlock with "[-HΦ Hj]"); iFrame.
-    { iFrame "Hinv"; eauto. }
+    { iFrame "Hlockinv"; eauto. }
     iIntros "!> _".
     wp_ret. by iApply "HΦ".
   Qed.
 
-  (* TODO: stop 'compile' from getting unfolded by the various Iris tactics. *)
-
-  (* TODO: this induction argument is completely generic; so should be bundled
-     for arbitrary layers.  The important points are to show triples for each
-     prim op compilation with some common invariant (here, DBInv) which must
-     be Persistent and must imply source_ctx for some ρ. *)
-  Lemma induction_refinement {T1 T2} j K `{LanguageCtx DB.Op T1 T2 DB.l K} (e: proc DB.Op T1):
-    j ⤇ K e ∗ DBInv ⊢ WP StatDb.Impl.impl.(compile) e {{ v, j ⤇ K (Ret v) }}.
+  Lemma init_mem_split: 
+    (([∗ map] i↦v ∈ init_zero, i m↦ v) -∗
+                                lock_addr m↦ 0 ∗ sum_addr m↦ 0 ∗ count_addr m↦ 0)%I.
   Proof.
-    iIntros "(Hj&#Hinv)".
-    iInduction e as [] "IH" forall (j T2 K H0).
-    - destruct op.
-      * iApply (add_refinement j K with "[$]"); eauto.
-      * iApply (avg_refinement j K with "[$]"); eauto.
-    - wp_ret. eauto.
-    - wp_bind.
-      iApply wp_wand_l. iSplitL ""; last first.
-      * iApply ("IH1" $! _ _ (fun x => K (Bind x p2)) with "[] Hj"); try iFrame.
-        { iPureIntro. apply comp_ctx; auto. apply _. }
-      * iIntros (?) "Hj".
-        iMod (ghost_step_bind_ret with "Hj []") as "Hj".
-        { set_solver+. }
-        { iDestruct "Hinv" as "($&?)". }
-        iApply "IH"; auto.
-    - iLöb as "IHloop" forall (init).
-      iMod (ghost_step_loop with "Hj []") as "Hj".
-      { set_solver+. }
-      { iDestruct "Hinv" as "($&?)". }
-      wp_loop.
-      iApply wp_wand_l.
-      iSplitL ""; last first.
-      * rewrite /loop1. simpl.
-        iApply ("IH" $! _ _ _ (fun x => K (Bind x
-                               (fun out => match out with
-                               | ContinueOutcome x => Loop body x
-                               | DoneWithOutcome r => Ret r
-                               end))) with "[] Hj")%proc.
-        { iPureIntro. apply comp_ctx; auto. apply _. }
-      * iIntros (out) "Hj".
-        destruct out.
-        ** iNext.
-           iMod (ghost_step_bind_ret with "Hj []") as "Hj".
-           { set_solver+. }
-           { iDestruct "Hinv" as "($&?)". }
-             by iApply "IHloop".
-        ** iNext.
-           iMod (ghost_step_bind_ret with "Hj []") as "Hj".
-           { set_solver+. }
-           { iDestruct "Hinv" as "($&?)". }
-           by wp_ret.
-   - iMod (ghost_step_spawn with "Hj []") as "(Hj&Hj')".
-     { set_solver+. }
-     { iDestruct "Hinv" as "($&?)". }
-     iDestruct "Hj'" as (j') "Hj'".
-     iApply (wp_spawn with "[Hj'] [Hj]").
-     { iNext. iApply wp_wand_l; iSplitL ""; last first.
-       { iApply ("IH" $! _ _ (fun x => x)); first (iPureIntro; apply _).
-         iFrame. }
-       eauto. }
-     eauto.
+    iIntros "Hmem".
+    rewrite (big_opM_delete _ _ 0 0); last first.
+    { rewrite /ExMach.mem_state. apply init_zero_lookup_lt_zero. rewrite /size. lia. }
+    rewrite (big_opM_delete _ _ 1 0); last first.
+    { rewrite /ExMach.mem_state.
+      rewrite lookup_delete_ne; last auto.
+      apply init_zero_lookup_lt_zero. rewrite /size. lia. }
+    rewrite (big_opM_delete _ _ 2 0); last first.
+    { rewrite /ExMach.mem_state.
+      rewrite lookup_delete_ne; last auto.
+      rewrite lookup_delete_ne; last auto.
+      apply init_zero_lookup_lt_zero. rewrite /size. lia. }
+    iDestruct "Hmem" as "(?&?&?&_)".
+    iFrame.
   Qed.
 
 End refinement_triples.
+
+Section refinement.
+
+  Definition helperΣ : gFunctors := #[GFunctor (authR (optionUR (exclR (listC natC))))].
+  Instance subG_helperΣ : subG helperΣ Σ → inG Σ (authR (optionUR (exclR (listC natC)))).
+  Proof. solve_inG. Qed.
+  
+  Definition myΣ : gFunctors := #[Adequacy.exmachΣ; @cfgΣ DB.Op DB.l; lockΣ; helperΣ].
+  Existing Instance subG_cfgPreG.
+  
+  Definition init_absr σ1a σ1c :=
+    ExMach.l.(initP) σ1c ∧ DB.l.(initP) σ1a.
+
+
+  Import ExMach.
+  Lemma exmach_crash_refinement_seq {T} σ1c σ1a (es: proc_seq DB.Op T) :
+    init_absr σ1a σ1c →
+    ¬ proc_exec_seq DB.l es (rec_singleton (Ret ())) σ1a Err →
+    ∀ σ2c res, ExMach.l.(proc_exec_seq) (compile_proc_seq StatDb.Impl.impl es)
+                                        (rec_singleton recv) σ1c (Val σ2c res) →
+    ∃ σ2a, DB.l.(proc_exec_seq) es (rec_singleton (Ret tt)) σ1a (Val σ2a res).
+  Proof.
+    eapply (exmach_crash_refinement_seq) with
+        (Σ := myΣ)
+        (exec_inv := fun H1 H2 => (∃ ρ, @DBInv myΣ H2 _ H1 _ ρ)%I)
+        (crash_inv := fun H1 H2 =>(∃ ρ, @CrashInv myΣ H2 H1 ρ)%I)
+        (exec_inner := fun H1 H2 => (∃ v, lock_addr m↦ v ∗
+            (∃ γ, (⌜ v = 0  ⌝-∗ @DBLockInv myΣ H2 _ γ) ∗ @DBInnerInv _ _ _ γ))%I)
+        (crash_inner := fun H1 H2 => (@DBCrashInner myΣ H2 H1)%I)
+        (E := nclose sourceN).
+    { apply _. }
+    { apply _. }
+    { intros. apply _. }
+    { intros. apply _. }
+    { set_solver+. }
+    { intros. iIntros "(?&HDB)". iDestruct "HDB" as (ρ) "HDB". destruct op.
+      - iApply (add_refinement with "[$]"). iNext. iIntros (?) "H". iApply "H".
+      - iApply (avg_refinement with "[$]"). iNext. iIntros (?) "H". iApply "H".
+    }
+    { intros. iIntros "H". iDestruct "H" as (ρ) "(?&?)". eauto. }
+    { intros. iIntros "H". iDestruct "H" as (ρ) "(#Hctx&#Hinv)".
+      wp_ret. iInv "Hinv" as (l) ">(?&?&?&?)" "_".
+      rewrite /source_inv.
+      iMod (own_alloc (● (Excl' nil) ⋅ ◯ (Excl' nil))) as (γ2) "[Hauth Hfrag]".
+      { by eauto. }
+      iApply (fupd_mask_weaken _ _).
+      { solve_ndisj. }
+      iExists l, nil. iFrame.
+      iSplitL "".
+      { iPureIntro; econstructor. }
+      iClear "Hctx Hinv".
+      iIntros (???) "(#Hctx&Hstate)".
+      rewrite /DBLockInv.
+      iModIntro. iExists _. iFrame. iExists γ2. iSplitR "Hauth Hstate"; iIntros; iExists nil; iFrame.
+    }
+    { intros ?? (H&?). inversion H. subst. eapply ExMach.init_state_wf. }
+    { intros ??? (H&Hinit) ??. inversion H. inversion Hinit. subst.
+      iIntros "(Hmem&?&#?&Hstate)".
+      iMod (own_alloc (● (Excl' nil) ⋅ ◯ (Excl' nil))) as (γ2) "[Hauth Hfrag]".
+      { clear. by eauto. }
+      iPoseProof (init_mem_split with "Hmem") as "(?&?&?)".
+      iModIntro. iExists _. iFrame. iExists γ2. iSplitR "Hauth Hstate"; iIntros; iExists nil; iFrame.
+    }
+    { intros. iIntros "H". iDestruct "H" as (ρ) "(#Hctx&#Hinv)".
+      iDestruct "Hinv" as (γ1 γ2) "(Hlock&#Hinv)".
+      rewrite /DBCrashInner.
+      iInv "Hinv" as ">Hopen" "_".
+      iDestruct "Hopen" as (l) "(?&?)".
+      iApply fupd_mask_weaken; first by solve_ndisj.
+      iIntros (?) "Hmem".
+      iModIntro. iExists l; iFrame.
+      iPoseProof (@init_mem_split with "Hmem") as "(?&?&?)".
+      iFrame.
+    }
+    { intros. iIntros "H". iDestruct "H" as (ρ) "(#Hctx&#Hinv)".
+      rewrite /DBCrashInner.
+      iInv "Hinv" as ">Hopen" "_".
+      iDestruct "Hopen" as (l) "(?&?)".
+      iApply fupd_mask_weaken; first by solve_ndisj.
+      iIntros (?) "Hmem".
+      iModIntro. iExists l. iFrame.
+      iPoseProof (@init_mem_split with "Hmem") as "(?&?&?)".
+      iFrame.
+    }
+    { intros. iIntros "H". iDestruct "H" as "(Hinv&#Hsrc)".
+      iDestruct "Hinv" as (invG) "Hinv".
+      rewrite /DBCrashInner/CrashInv.
+      iDestruct "Hinv" as (l) "(?&?)".
+      iMod (@inv_alloc myΣ (exm_invG) iN _ DBCrashInner with "[-]").
+      { iNext. iExists l; iFrame. }
+      iModIntro. iExists _. iFrame "Hsrc". auto.
+    }
+    { intros. iIntros "H". iDestruct "H" as "(Hinv&#Hsrc)".
+      iDestruct "Hinv" as (invG v) "Hinv".
+      iDestruct "Hinv" as "(?&Hinv)".
+      iDestruct "Hinv" as (γ2) "(Hlock&Hinner)".
+      iMod (@lock_init myΣ (ExMachG _ (exm_invG) (exm_mem_inG) (exm_disk_inG)) _ lN
+                       lock_addr _ (DBLockInv γ2) with "[$] [-Hinner]") as (γ1) "H".
+      { iFrame. }
+      iMod (@inv_alloc myΣ (exm_invG) iN _ (DBInnerInv γ2) with "[Hinner]").
+      { iFrame. }
+      iModIntro. rewrite /DBInv. iExists cfg. iFrame "Hsrc". iExists γ1, γ2. iFrame.
+    }
+    { iIntros (??) "H".
+      iDestruct "H" as (?) "(?&H)".
+      iDestruct "H" as (??) "(?&Hinv)".
+      iInv "Hinv" as (l') ">(Htok&Hsource)" "_".
+      iApply fupd_mask_weaken; first by solve_ndisj.
+      iExists _; eauto.
+    }
+    { iIntros (??) "H".
+      iDestruct "H" as (?) "(?&H)".
+      iDestruct "H" as (γ1 γ2) "(Hlock&Hinv)".
+      iInv "Hinv" as (l') ">(Htok&Hsource)" "_".
+      iMod (lock_crack with "Hlock") as ">H"; first by solve_ndisj.
+      iDestruct "H" as (v) "(?&?)".
+      iApply fupd_mask_weaken; first by solve_ndisj.
+      iExists _; eauto.
+      iFrame. iIntros (???) "(?&?)".
+      iModIntro.
+      iExists v. iFrame. iExists γ2. iFrame. 
+      iExists _. iFrame.
+    }
+  Qed.
+
+End refinement.
